lean/Och/Std.lean
@@ -2,6 +2,7 @@ import Och.Std.Unit
 import Och.Std.Bool
 import Och.Std.DBool
 import Och.Std.Nat
+import Och.Std.DNat
 import Och.Std.Pair
 import Och.Std.Sigma
 import Och.Std.Array
